Other/1Part.lean
@@ -1,0 +1,129 @@
+-- from https://arxiv.org/pdf/1810.08380
+import Mathlib.Tactic.Use
+import Mathlib.Data.Nat.Pairing
+
+namespace PartRec
+
+-- 4.1 The Partity monad
+
+/--
+We define `Part α` as a dependent pair of a proposition `p`
+and a function `p → α`. This is equivalent to `Σ' p : Prop, (p → α)`.
+-/
+-- same as mathlib Part
+structure Part.{u} (α : Type u) : Type u where
+  /-- The domain of a Part value -/
+  Dom : Prop
+  /-- Extract a value from a Part value given a proof of `Dom` -/
+  get : Dom → α
+
+namespace Part
+
+/-- The `pure` operation for the `Part` monad. -/
+@[simp] def pure {α : Type u} (a : α) : Part α :=
+  ⟨True, fun _ => a⟩
+
+/-- The `bind` operation. -/
+@[simp] def bind {α β : Type u} (p : Part α) (f : α → Part β) : Part β :=
+  ⟨(∀ h : p.Dom, (f (p.get h)).Dom) ∧ p.Dom, fun h =>
+    (f (p.get h.right)).get (h.left h.right)⟩
+
+/-- `map` operation to complete the `Monad` structure. -/
+@[simp] def map {α β : Type u} (f : α → β) (p : Part α) : Part β :=
+  ⟨p.Dom, f ∘ p.get⟩
+
+instance : Monad Part where
+  pure := pure
+  bind := bind
+  map := map
+
+/-- Undefined value. -/
+@[simp] def bottom {α : Type u} : Part α :=
+  ⟨False, False.elim⟩
+
+notation "⊥" => bottom
+
+instance {α : Type u} : Inhabited (Part α) := ⟨bottom⟩
+
+/-- Relational membership for `Part` (a ∈ p). -/
+instance {α : Type u} : Membership α (Part α) where
+  mem p a := ∃ h : p.Dom, p.get h = a
+
+/-- Theorem relating bind and membership. -/
+theorem mem_bind {α β : Type u} (p : Part α) (f : α → Part β) (b : β) :
+    b ∈ p >>= f ↔ ∃ a ∈ p, b ∈ f a := by
+  constructor
+  · rintro ⟨h_exist, h_eq⟩
+    use p.get h_exist.right
+    constructor
+    · exact ⟨h_exist.right, rfl⟩
+    · exact ⟨h_exist.left h_exist.right, h_eq⟩
+  · rintro ⟨a, ⟨h1, rfl⟩, ⟨h2, h_eq⟩⟩
+    exact ⟨⟨fun _ => h2, h1⟩, h_eq⟩
+
+end Part
+
+
+-- Notation for Part functions
+-- https://github.com/digama0/mathlib-ITP2019/blob/5cbd0362e04e671ef5db1284870592af6950197c/src/data/pfun.lean#L297
+-- https://loogle.lean-lang.org/?q=%3Fa+-%3E+Part+%3Fa
+-- !!!!!! https://github.com/leanprover-community/mathlib4/blob/878dc46fb98bc3a247541bd4d109dd65cd0092bc/Mathlib/Data/PFun.lean#L59-L62
+infixr:50 " ⇀ " => fun α β => α → Part β
+
+-- Computable unbounded recursion (`fix`)
+-- https://github.com/digama0/mathlib-ITP2019/blob/5cbd0362e04e671ef5db1284870592af6950197c/src/data/pfun.lean#L416-L422
+-- https://github.com/leanprover-community/mathlib4/blob/9dc39333aa89d5be59e8d7698237b31e496cf4ea/Mathlib/Data/PFun.lean#L216
+opaque fix {α β : Type u} (f : α ⇀ Sum β α) : α ⇀ β
+
+-- theorem mem_fix_iff {f : α →. β ⊕ α} {a : α} {b : β} :
+--     b ∈ f.fix a ↔ Sum.inl b ∈ f a ∨ ∃ a', Sum.inr a' ∈ f a ∧ b ∈ f.fix a' :=
+axiom mem_fix {α β : Type u} (f : α ⇀ Sum β α) (a : α) (b : β) :
+  b ∈ fix f a ↔ Sum.inl b ∈ f a ∨ ∃ a', Sum.inr a' ∈ f a ∧ b ∈ fix f a'
+
+
+-- Figure 5: The definition of Part recursive on Nat in Lean
+
+/-- Helper for prec that maps an uncurried function handling Nat.unpairs. -/
+def Nat.unpaired (h : Nat → Nat → Part Nat) : Nat ⇀ Nat :=
+  fun n => let n' := Nat.unpair n; h n'.1 n'.2
+
+/--
+The minimization operator `find p = µn. p(n)`, which finds the smallest
+value satisfying the (Part) boolean predicate `p`.
+-/
+-- https://github.com/leanprover-community/mathlib4/blob/878dc46fb98bc3a247541bd4d109dd65cd0092bc/Mathlib/Computability/Partrec.lean#L89-L93
+def find (p : Nat ⇀ Bool) : Part Nat :=
+  fix (fun n =>
+    p n >>= fun b =>
+      if b then pure (Sum.inl n) else pure (Sum.inr (n + 1))) 0
+
+-- this is not find, bc this is total search
+-- def Nat.find{p : ℕ → Prop} [DecidablePred p] (H : ∃ (n : ℕ), p n) : ℕ
+-- def PNat.find{p : ℕ+ → Prop} [DecidablePred p] (h : ∃ (n : ℕ+), p n) : ℕ+
+
+-- https://github.com/leanprover-community/mathlib4/blob/878dc46fb98bc3a247541bd4d109dd65cd0092bc/Mathlib/Computability/Partrec.lean#L160
+inductive Partrec : (Nat ⇀ Nat) → Prop
+  | zero : Partrec (fun _ => pure 0)
+  | succ : Partrec (fun n => pure (n + 1))
+  | left : Partrec (fun n => pure n)
+  | right : Partrec (fun n => pure n)
+  | pair {f g} : Partrec f → Partrec g →
+      Partrec (fun n =>
+        f n >>= fun a =>
+        g n >>= fun b =>
+        pure (Nat.pair a b))
+  | comp {f g} : Partrec f → Partrec g →
+      Partrec (fun n => g n >>= f)
+  | prec {f g} : Partrec f → Partrec g →
+      Partrec (Nat.unpaired (fun a n =>
+        Nat.recOn n
+          (f a)
+          (fun y IH =>
+            IH >>= fun i =>
+            g (Nat.pair a (Nat.pair y i)))))
+  | find {f} : Partrec f →
+      Partrec (fun a =>
+        find (fun n =>
+          (fun m => m == 0) <$> f (Nat.pair a n)))
+
+end PartRec
