Plfl/Init/Lemmas.lean
@@ -1,0 +1,8 @@
+module
+
+public section
+theorem congr_arg₃
+(f : α → β → γ → δ) {x x' : α} {y y' : β} {z z' : γ}
+(hx : x = x') (hy : y = y') (hz : z = z')
+: f x y z = f x' y' z'
+:= by subst hx hy hz; rfl
